seal wp and pvs

program_logic/pviewshifts.v
@@ -9,8 +9,7 @@ Local Hint Extern 10 (✓{_} _) =>
   | H : wsat _ _ _ _ |- _ => apply wsat_valid in H; last omega
   end; solve_validN.
 
-(* TODO: Consider sealing this, like all the definitions in upred.v. *)
-Program Definition pvs {Λ Σ} (E1 E2 : coPset) (P : iProp Λ Σ) : iProp Λ Σ :=
+Program Definition pvs_def {Λ Σ} (E1 E2 : coPset) (P : iProp Λ Σ) : iProp Λ Σ :=
   {| uPred_holds n r1 := ∀ rf k Ef σ,
        0 < k ≤ n → (E1 ∪ E2) ∩ Ef = ∅ →
        wsat k (E1 ∪ Ef) σ (r1 ⋅ rf) →
@@ -25,7 +24,12 @@ Next Obligation.
   exists (r' ⋅ r3); rewrite -assoc; split; last done.
   apply uPred_weaken with k r'; eauto using cmra_included_l.
 Qed.
-Arguments pvs {_ _} _ _ _%I : simpl never.
+
+Definition pvs_aux : { x | x = @pvs_def }. by eexists. Qed.
+Definition pvs := proj1_sig pvs_aux.
+Definition pvs_eq : @pvs = @pvs_def := proj2_sig pvs_aux.
+
+Arguments pvs {_ _} _ _ _%I.
 Instance: Params (@pvs) 4.
 
 Notation "|={ E1 , E2 }=> Q" := (pvs E1 E2 Q%I)
@@ -43,6 +47,7 @@ Transparent uPred_holds.
 
 Global Instance pvs_ne E1 E2 n : Proper (dist n ==> dist n) (@pvs Λ Σ E1 E2).
 Proof.
+  rewrite pvs_eq.
   intros P Q HPQ; split=> n' r1 ??; simpl; split; intros HP rf k Ef σ ???;
     destruct (HP rf k Ef σ) as (r2&?&?); auto;
     exists r2; split_and?; auto; apply HPQ; eauto.
@@ -52,18 +57,18 @@ Proof. apply ne_proper, _. Qed.
 
 Lemma pvs_intro E P : P ⊑ |={E}=> P.
 Proof.
-  split=> n r ? HP rf k Ef σ ???; exists r; split; last done.
+  rewrite pvs_eq. split=> n r ? HP rf k Ef σ ???; exists r; split; last done.
   apply uPred_weaken with n r; eauto.
 Qed.
 Lemma pvs_mono E1 E2 P Q : P ⊑ Q → (|={E1,E2}=> P) ⊑ (|={E1,E2}=> Q).
 Proof.
-  intros HPQ; split=> n r ? HP rf k Ef σ ???.
+  rewrite pvs_eq. intros HPQ; split=> n r ? HP rf k Ef σ ???.
   destruct (HP rf k Ef σ) as (r2&?&?); eauto.
   exists r2; eauto using uPred_in_entails.
 Qed.
 Lemma pvs_timeless E P : TimelessP P → (▷ P) ⊑ (|={E}=> P).
 Proof.
-  rewrite uPred.timelessP_spec=> HP.
+  rewrite pvs_eq uPred.timelessP_spec=> HP.
   uPred.unseal; split=>-[|n] r ? HP' rf k Ef σ ???; first lia.
   exists r; split; last done.
   apply HP, uPred_weaken with n r; eauto using cmra_validN_le.
@@ -71,19 +76,19 @@ Qed.
 Lemma pvs_trans E1 E2 E3 P :
   E2 ⊆ E1 ∪ E3 → (|={E1,E2}=> |={E2,E3}=> P) ⊑ (|={E1,E3}=> P).
 Proof.
-  intros ?; split=> n r1 ? HP1 rf k Ef σ ???.
+  rewrite pvs_eq. intros ?; split=> n r1 ? HP1 rf k Ef σ ???.
   destruct (HP1 rf k Ef σ) as (r2&HP2&?); auto.
 Qed.
 Lemma pvs_mask_frame E1 E2 Ef P :
   Ef ∩ (E1 ∪ E2) = ∅ → (|={E1,E2}=> P) ⊑ (|={E1 ∪ Ef,E2 ∪ Ef}=> P).
 Proof.
-  intros ?; split=> n r ? HP rf k Ef' σ ???.
+  rewrite pvs_eq. intros ?; split=> n r ? HP rf k Ef' σ ???.
   destruct (HP rf k (Ef∪Ef') σ) as (r'&?&?); rewrite ?(assoc_L _); eauto.
   by exists r'; rewrite -(assoc_L _).
 Qed.
 Lemma pvs_frame_r E1 E2 P Q : ((|={E1,E2}=> P) ★ Q) ⊑ (|={E1,E2}=> P ★ Q).
 Proof.
-  uPred.unseal; split; intros n r ? (r1&r2&Hr&HP&?) rf k Ef σ ???.
+  rewrite pvs_eq. uPred.unseal; split; intros n r ? (r1&r2&Hr&HP&?) rf k Ef σ ???.
   destruct (HP (r2 ⋅ rf) k Ef σ) as (r'&?&?); eauto.
   { by rewrite assoc -(dist_le _ _ _ _ Hr); last lia. }
   exists (r' ⋅ r2); split; last by rewrite -assoc.
@@ -91,7 +96,7 @@ Proof.
 Qed.
 Lemma pvs_openI i P : ownI i P ⊑ (|={{[i]},∅}=> ▷ P).
 Proof.
-  uPred.unseal; split=> -[|n] r ? Hinv rf [|k] Ef σ ???; try lia.
+  rewrite pvs_eq. uPred.unseal; split=> -[|n] r ? Hinv rf [|k] Ef σ ???; try lia.
   apply ownI_spec in Hinv; last auto.
   destruct (wsat_open k Ef σ (r ⋅ rf) i P) as (rP&?&?); auto.
   { rewrite lookup_wld_op_l ?Hinv; eauto; apply dist_le with (S n); eauto. }
@@ -100,7 +105,7 @@ Proof.
 Qed.
 Lemma pvs_closeI i P : (ownI i P ∧ ▷ P) ⊑ (|={∅,{[i]}}=> True).
 Proof.
-  uPred.unseal; split=> -[|n] r ? [? HP] rf [|k] Ef σ ? HE ?; try lia.
+  rewrite pvs_eq. uPred.unseal; split=> -[|n] r ? [? HP] rf [|k] Ef σ ? HE ?; try lia.
   exists ∅; split; [done|].
   rewrite left_id; apply wsat_close with P r.
   - apply ownI_spec, uPred_weaken with (S n) r; auto.
@@ -111,7 +116,7 @@ Qed.
 Lemma pvs_ownG_updateP E m (P : iGst Λ Σ → Prop) :
   m ~~>: P → ownG m ⊑ (|={E}=> ∃ m', ■ P m' ∧ ownG m').
 Proof.
-  intros Hup%option_updateP'.
+  rewrite pvs_eq. intros Hup%option_updateP'.
   uPred.unseal; split=> -[|n] r ? /ownG_spec Hinv rf [|k] Ef σ ???; try lia.
   destruct (wsat_update_gst k (E ∪ Ef) σ r rf (Some m) P) as (m'&?&?); eauto.
   { apply cmra_includedN_le with (S n); auto. }
@@ -121,7 +126,7 @@ Lemma pvs_ownG_updateP_empty `{Empty (iGst Λ Σ), !CMRAIdentity (iGst Λ Σ)}
     E (P : iGst Λ Σ → Prop) :
   ∅ ~~>: P → True ⊑ (|={E}=> ∃ m', ■ P m' ∧ ownG m').
 Proof.
-  intros Hup; uPred.unseal; split=> -[|n] r ? _ rf [|k] Ef σ ???; try lia.
+  rewrite pvs_eq. intros Hup; uPred.unseal; split=> -[|n] r ? _ rf [|k] Ef σ ???; try lia.
   destruct (wsat_update_gst k (E ∪ Ef) σ r rf ∅ P) as (m'&?&?); eauto.
   { apply cmra_empty_leastN. }
   { apply cmra_updateP_compose_l with (Some ∅), option_updateP with P;
@@ -130,7 +135,7 @@ Proof.
 Qed.
 Lemma pvs_allocI E P : ¬set_finite E → ▷ P ⊑ (|={E}=> ∃ i, ■ (i ∈ E) ∧ ownI i P).
 Proof.
-  intros ?; rewrite /ownI; uPred.unseal.
+  rewrite pvs_eq. intros ?; rewrite /ownI; uPred.unseal.
   split=> -[|n] r ? HP rf [|k] Ef σ ???; try lia.
   destruct (wsat_alloc k E Ef σ rf P r) as (i&?&?&?); auto.
   { apply uPred_weaken with n r; eauto. }
